STLCWA.v
@@ -1,0 +1,19 @@
+Module STLCARITH.
+
+Inductive ty : Type :=
+    | TArrow : ty -> ty -> ty
+    | TNat : ty.
+
+Inductive tm : Type :=
+    | tvar : id -> tm 
+    | tapp : tm -> tm -> tm
+    | tabs : id -> ty -> tm -> tm 
+    | tnat : nat -> tm 
+    | tsucc : tm -> tm 
+    | tpred : tm -> tm 
+    | tmult : tm -> tm -> tm 
+    | tif0 : tm -> tm -> tm -> tm.
+
+(*Weak Typing. 0 as False, others are true.*)
+
+In
